dist/SizeClassSelection.h
@@ -6,6 +6,10 @@
 
 #include "krmllib.h"
 
+extern krml_checked_int_t SizeClassSelection__n;
+
+extern krml_checked_int_t SizeClassSelection__k;
+
 uint32_t SizeClassSelection_log2u64(uint64_t x);
 
 uint32_t SizeClassSelection_inv_impl(uint32_t x);
