src/Constants.fst
@@ -1,17 +1,20 @@
 module Constants
 
 module U32 = FStar.UInt32
+module US = FStar.SizeT
 
 open FStar.Mul
+open Prelude
 
 // LATER: code could be improved so that this value is not hardcoded anymore
 inline_for_extraction
 let page_size: U32.t = 4096ul
 
-noextract
-let min_sc = 64
-noextract
-let max_sc = U32.v page_size
+//inline_for_extraction
+let max_slab_size: U32.t = 131072ul
+
+//inline_for_extraction
+//let max_slab_size: US.t = US.uint32_to_sizet max_slab_size'
 
 // TODO: this could be improved
 // currently does not support size classes
@@ -24,13 +27,53 @@ let max_sc = U32.v page_size
 // note: this mechanism does not rely on any loop!
 inline_for_extraction noextract
 let sc = x:U32.t{
-  (
-    U32.eq x 16ul \/
-    U32.eq x 32ul \/
-    (min_sc <= U32.v x /\ U32.v x <= max_sc)
-  ) /\
+  //(
+  //  U32.eq x 16ul \/
+  //  U32.eq x 32ul \/
+  //  (min_sc <= U32.v x /\ U32.v x <= max_sc)
+  //) /\
   // https://www.intel.com/content/dam/develop/external/us/en/documents/mpx-linux64-abi.pdf
   // allocated arrays should have alignment of at least 16 bytes,
   // allowing use of SSE instructions
-  (U32.v x % 16 == 0)
+  U32.v x > 0 /\
+  (U32.v x) % 16 == 0 /\
+  U32.fits (U32.v x * 256)
+}
+
+inline_for_extraction noextract
+let sc_p (x: sc) (y: U32.t)
+  =
+  // bitmap handling: 256 bits max
+  // supported number of slots: any value in S \cup {128, 256},
+  // where S is the integer interval [[1, 64]]
+  U32.v y <= 256 * U32.v x /\
+  (
+    // x = 16
+    (U32.eq y (U32.mul x 256ul)) \/
+    //(U32.div y 256ul)) \/
+    // x = 32
+    (U32.eq y (U32.mul x 128ul)) \/
+    //(U32.div y 128ul)) \/
+    // x >= 64
+    (U32.lte y (U32.mul x 64ul))
+  ) /\
+  // why is this useful?
+  U32.v y <= U32.v max_slab_size /\
+  // one slot fits on a slab
+  U32.v x <= U32.v y /\
+  // for guard pages + quarantined pages: permission management is done using pages
+  (U32.v y) % (U32.v page_size) == 0 /\
+  // alignement
+  (U32.v max_slab_size) % (U32.v y) == 0 /\
+  // small sizeclasses: no page boundary crossing, useful in SizeClass.fst
+  // to retrieve alignment
+  (U32.v x <= 4096 ==> U32.v y <= 4096) /\
+  True
+
+type sc_full' = {
+  sc: sc;
+  slab_size: v:U32.t{sc_p sc v};
+  md_max: v:US.t{
+    US.fits (U32.v slab_size * US.v v)
+  };
 }
