src/Quarantine.fst
@@ -3,33 +3,33 @@ module Quarantine
 open Constants
 open Config
 
-let quarantine_slab arr =
+let quarantine_slab sc arr =
   if enable_quarantine_trap
-  then trap_array arr
+  then trap_array sc arr
   else A.varray arr
 
-let mmap_trap_quarantine arr len =
+let mmap_trap_quarantine sc arr len =
   if enable_quarantine_trap then (
     if enable_quarantine_strict_trap then (
-      mmap_strict_trap arr len
+      mmap_strict_trap (G.hide sc) arr len
     ) else (
-      mmap_trap arr len
+      mmap_trap (G.hide sc) arr len
     );
-    change_equal_slprop (trap_array arr) (quarantine_slab arr)
+    change_equal_slprop (trap_array sc arr) (quarantine_slab sc arr)
   ) else (
     noop ();
-    change_equal_slprop (A.varray arr) (quarantine_slab arr)
+    change_equal_slprop (A.varray arr) (quarantine_slab sc arr)
   )
 
-let mmap_untrap_quarantine arr len =
+let mmap_untrap_quarantine sc arr len =
   if enable_quarantine_trap then (
-    change_equal_slprop (quarantine_slab arr) (trap_array arr);
+    change_equal_slprop (quarantine_slab sc arr) (trap_array sc arr);
     if enable_quarantine_strict_trap then (
-      mmap_strict_untrap arr len
+      mmap_strict_untrap sc arr len
     ) else (
-      mmap_untrap arr len
+      mmap_untrap sc arr len
     )
   ) else (
     noop ();
-    change_equal_slprop (quarantine_slab arr) (A.varray arr)
+    change_equal_slprop (quarantine_slab sc arr) (A.varray arr)
   )
