src/Mman.fst
@@ -35,7 +35,7 @@ assume val mmap_u8_init (len: US.t)
       A.length r == US.v len /\
       A.is_full_array r /\
       A.asel r h1 == Seq.create (US.v len) U8.zero /\
-      array_u8_alignment r page_size
+      array_u8_alignment r max_slab_size
     )
 
 assume val mmap_u64_init (len: US.t)
